Fairly extensive modifications to give integerTheory two division functions (and each gets a corresponding mod function too).  They are int_div (int_mod) and int_quot (int_rem).  All are abbreviated by the printer-parser:   int_mod  : %   int_div  : /   int_rem  : rem   int_quot : quot The behaviour is as for the SML constants of the Basis Library's Integer structure.  Most theorems about one function have analogous theorems in the other camp.  Cooper's algorithm modified to work with int_div and int_mod.  I haven't made it work over the other pair, though I probably should at some stage.

src/integer/CooperShell.sml
@@ -1,4 +1,4 @@
-structure CooperShell :> CooperShell = 
+structure CooperShell :> CooperShell =
 struct
 
 open HolKernel boolLib integerTheory Parse
@@ -680,9 +680,7 @@ fun elim_div_mod0 t = let
                  div_nzero
   in
     UNBETA_CONV to_elim THENC REWR_CONV rwt THENC
-    REWRITE_CONV [abs_div] THENC REWRITE_CONV [INT_ABS_LT, INT_ABS_LE] THENC
-    STRIP_QUANT_CONV (RAND_CONV (RAND_CONV (RAND_CONV BETA_CONV))) THENC
-    push_in_exists
+    STRIP_QUANT_CONV (RAND_CONV (FORK_CONV (REDUCE_CONV, BETA_CONV)))
   end
 in
   EVERY_QCONV (map elim_t divmods) t
